Transfer more theorems semi-automatically to monoid as type theory

examples/algebra/aat/aatmonoidScript.sml
@@ -1,6 +1,6 @@
 open HolKernel Parse boolLib bossLib;
 
-open monoidTheory transferTheory transferLib
+open monoidTheory monoidOrderTheory transferTheory transferLib
 
 val _ = new_theory "aatmonoid";
 
@@ -72,6 +72,12 @@ Theorem tmonoid_repabs_id:
   Monoid m ∧ oodf m.carrier m.op = m.op ⇒ monoid_REP (monoid_ABS m) = m
 Proof
   strip_tac >> irule (#repabs_pseudo_id mrec) >> simp[fullmonoid_def]
+QED
+
+Theorem Monoid_monoid_REP[simp]:
+  !m. Monoid (monoid_REP m)
+Proof
+  simp[FORALL_tmonoid, tmonoid_repabs_id]
 QED
 
 Theorem tmop_relates[transfer_rule]:
@@ -213,6 +219,358 @@ Proof
   simp[AbelianMonoid_def, FUN_REL_def, MTR_def]
 QED
 
+Definition FiniteAbelianMonoid_def:
+  FiniteAbelianMonoid (m:α monoid) ⇔ FiniteMonoid m ∧ AbelianMonoid m
+End
 
+Theorem FiniteAbelianMonoid_relates[transfer_rule]:
+  (MTR |==> (=)) FiniteAbelianMonoid FiniteAbelianMonoid
+Proof
+  simp[FiniteAbelianMonoid_def, monoidTheory.FiniteAbelianMonoid_def,
+       FUN_REL_def, FiniteMonoid_def, MTR_def, AbelianMonoid_def] >>
+  metis_tac[]
+QED
+
+Theorem FiniteAbelianMonoid_def_alt:
+  ∀m. FiniteAbelianMonoid m ⇔
+        FiniteMonoid m ∧
+        ∀x y. x ∈ tmcarrier m ∧ y ∈ tmcarrier m ⇒ tmop m x y = tmop m y x
+Proof
+  xfer_back_tac[] >> simp[monoidTheory.FiniteAbelianMonoid_def_alt]
+QED
+
+Theorem monoid_carrier_nonempty[simp]:
+  ∀m. tmcarrier m <> {}
+Proof
+  xfer_back_tac [] >> simp[monoid_carrier_nonempty]
+QED
+
+Definition monoid_exp_def:
+  monoid_exp m x n = monoid$monoid_exp (monoid_REP m) x n
+End
+
+Theorem monoid_exp_relates[transfer_rule]:
+  (MTR |==> (=) |==> (=) |==> (=)) monoid_exp monoid_exp
+Proof
+  simp[FUN_REL_def, monoid_exp_def, MTR_def]
+QED
+
+Theorem monoid_exp_thm[simp]:
+  !m x. monoid_exp m x 0 = tmid m /\
+        !n. monoid_exp m x (SUC n) = tmop m x (monoid_exp m x n)
+Proof
+  xfer_back_tac []  >> simp[]
+QED
+
+Theorem monoid_exp_FUNPOW:
+  !m x n. monoid_exp m x n = FUNPOW (tmop m x) n (tmid m)
+Proof
+  xfer_back_tac [] >> simp[monoidTheory.monoid_exp_def]
+QED
+
+Theorem monoid_exp_element[simp]:
+  !m x. x ∈ tmcarrier m ⇒ !n. monoid_exp m x n ∈ tmcarrier m
+Proof
+  xfer_back_tac [] >> simp[monoidTheory.monoid_exp_element]
+QED
+
+Theorem monoid_exp_1[simp]:
+  !m x. monoid_exp m x 1 = x
+Proof
+  rewrite_tac[arithmeticTheory.ONE, monoid_exp_thm] >>
+  simp[]
+QED
+
+Theorem monoid_id_exp[simp]:
+  !m n. monoid_exp m (tmid m) n = tmid m
+Proof
+  xfer_back_tac [] >> simp[monoidTheory.monoid_id_exp]
+QED
+
+Theorem monoid_comm_exp:
+  !m x y n.
+    tmop m x y = tmop m y x ⇒
+    tmop m (monoid_exp m x n) y = tmop m y (monoid_exp m x n)
+Proof
+  Induct_on ‘n’ >> simp[] >> metis_tac[tmonoid_assoc]
+QED
+
+Theorem monoid_exp_comm:
+  !m x n.
+    tmop m (monoid_exp m x n) x = tmop m x (monoid_exp m x n)
+Proof
+  Induct_on ‘n’ >> simp[] >> simp[GSYM tmonoid_assoc]
+QED
+
+Theorem monoid_comm_op_exp:
+  !m n x y. tmop m x y = tmop m y x ⇒
+            monoid_exp m (tmop m x y) n =
+            tmop m (monoid_exp m x n) (monoid_exp m y n)
+Proof
+  Induct_on ‘n’ >> simp[] >> rpt strip_tac >>
+  first_x_assum (drule_then strip_assume_tac) >> simp[] >>
+  metis_tac[monoid_exp_comm, tmonoid_assoc, monoid_comm_exp]
+QED
+
+Theorem monoid_comm_exp_exp:
+  !m n p x y. tmop m x y = tmop m y x ⇒
+              tmop m (monoid_exp m x n) (monoid_exp m y p) =
+              tmop m (monoid_exp m y p) (monoid_exp m x n)
+Proof
+  Induct_on ‘n’ >> simp[] >>
+  metis_tac[tmonoid_assoc, monoid_comm_exp]
+QED
+
+Theorem monoid_exp_add:
+  !m n p x.
+    monoid_exp m x (n + p) = tmop m (monoid_exp m x n) (monoid_exp m x p)
+Proof
+  Induct_on ‘n’ >> simp[arithmeticTheory.ADD_CLAUSES, tmonoid_assoc]
+QED
+
+Theorem monoid_exp_mult:
+  !m n p x.
+    monoid_exp m x (n * p) = monoid_exp m (monoid_exp m x n) p
+Proof
+  Induct_on ‘p’ >> simp[arithmeticTheory.MULT_CLAUSES, monoid_exp_add]
+QED
+
+Theorem monoid_exp_mult_comm:
+  !m x n p.
+    monoid_exp m (monoid_exp m x n) p = monoid_exp m (monoid_exp m x p) n
+Proof
+  metis_tac[arithmeticTheory.MULT_COMM, monoid_exp_mult]
+QED
+
+(* ----------------------------------------------------------------------
+    Finite monoids
+   ---------------------------------------------------------------------- *)
+
+Theorem finite_monoid_exp_not_distinct:
+  !m x. FiniteMonoid m /\ x ∈ tmcarrier m ⇒
+        ∃h k. monoid_exp m x h = monoid_exp m x k /\ h ≠ k
+Proof
+  xfer_back_tac [] >> simp[] >>
+  metis_tac[monoidTheory.finite_monoid_exp_not_distinct,
+            monoidTheory.FiniteMonoid_def]
+QED
+
+(* ----------------------------------------------------------------------
+    MITSET : iterating monoid operation over (finite) set of elements
+   ---------------------------------------------------------------------- *)
+
+Overload MITSET = “λm. ITSET (tmop m)”
+
+Theorem abelian_monoid_op_closure_comm_assoc_fun:
+  !m. AbelianMonoid m ⇒ closure_comm_assoc_fun (tmop m) (tmcarrier m)
+Proof
+  xfer_back_tac [] >>
+  simp[monoidTheory.abelian_monoid_op_closure_comm_assoc_fun]
+QED
+
+Theorem COMMUTING_MITSET_INSERT:
+  !m s. AbelianMonoid m /\ FINITE s /\ s ⊆ tmcarrier m ⇒
+        !b x. b ∈ tmcarrier m /\ x ∈ tmcarrier m ⇒
+              MITSET m (x INSERT s) b = MITSET m (s DELETE x) (tmop m x b)
+Proof
+  xfer_back_tac [] >> simp[COMMUTING_GITSET_INSERT]
+QED
+
+Theorem COMMUTING_MITSET_REDUCTION:
+  !m s. AbelianMonoid m /\ FINITE s /\ s ⊆ tmcarrier m ⇒
+        !b x. b ∈ tmcarrier m /\ x ∈ tmcarrier m ⇒
+              MITSET m s (tmop m x b) = tmop m x (MITSET m s b)
+Proof
+  xfer_back_tac [] >> simp[COMMUTING_GITSET_REDUCTION]
+QED
+
+Theorem COMMUTING_MITSET_RECURSES:
+  !m s. AbelianMonoid m /\ FINITE s /\ s ⊆ tmcarrier m ⇒
+        !b x. b ∈ tmcarrier m /\ x ∈ tmcarrier m ⇒
+              MITSET m (x INSERT s) b = tmop m x (MITSET m (s DELETE x) b)
+Proof
+  xfer_back_tac [] >> simp[COMMUTING_GITSET_RECURSES]
+QED
+
+Overload MPROD_SET = “λm s. MITSET m s (tmid m)”
+
+Theorem MPROD_SET_SING[simp]:
+  !m x. MPROD_SET m {x} = x
+Proof
+  simp[]
+QED
+
+Theorem MPROD_SET_PROPERTY:
+  !m s. AbelianMonoid m /\ FINITE s /\ s ⊆ tmcarrier m ⇒
+        MPROD_SET m s ∈ tmcarrier m
+Proof
+  xfer_back_tac [] >> simp[GSYM GPROD_SET_def, GPROD_SET_PROPERTY]
+QED
+
+Definition tmextend_def:
+  tmextend m = mkmonoid (extend (monoid_REP m))
+End
+
+Theorem tmextend_relates[transfer_rule]:
+  (MTR |==> MTR) extend tmextend
+Proof
+  simp[FUN_REL_def, MTR_def, tmextend_def] >>
+  strip_tac >> irule tmonoid_repabs_id >> simp[]
+QED
+
+Theorem tmextend_carrier[simp]:
+  !m. tmcarrier (tmextend m) = UNIV
+Proof
+  xfer_back_tac [] >> simp[]
+QED
+
+Theorem tmextend_id[simp]:
+  !m. tmid (tmextend m) = tmid m
+Proof
+  xfer_back_tac [] >> simp[]
+QED
+
+Theorem tmextend_op:
+  !m x y. x ∈ tmcarrier m /\ y ∈ tmcarrier m ⇒
+          tmop (tmextend m) x y = tmop m x y
+Proof
+  xfer_back_tac [] >> simp[extend_op]
+QED
+
+Definition period_def:
+  period m x k = monoidOrder$period (monoid_REP m) x k
+End
+
+Theorem period_relates[transfer_rule]:
+  (MTR |==> (=) |==> (=) |==> (<=>)) period period
+Proof
+  simp[FUN_REL_def, period_def, MTR_def]
+QED
+
+Definition order_def:
+  order m x = monoidOrder$order (monoid_REP m) x
+End
+
+Theorem order_relates[transfer_rule]:
+  (MTR |==> (=) |==> (=)) order order
+Proof
+  simp[FUN_REL_def, order_def, MTR_def]
+QED
+
+Overload tord[local] = “aatmonoid$order m”
+
+Theorem order_property:
+  !m x. monoid_exp m x (tord x) = tmid m
+Proof
+  xfer_back_tac [] >> simp[monoidOrderTheory.order_property]
+QED
+
+Theorem order_period:
+  !m x. 0 < tord x ⇒ period m x (tord x)
+Proof
+  xfer_back_tac [] >> simp[order_period]
+QED
+
+Theorem order_minimal:
+  !m x n. 0 < n /\ n < tord x ⇒ monoid_exp m x n <> tmid m
+Proof
+  xfer_back_tac [] >> simp[order_minimal]
+QED
+
+Theorem order_eq_0:
+  !m x. tord x = 0 ⇔ !n. 0 < n ==> monoid_exp m x n <> tmid m
+Proof
+  xfer_back_tac [] >> simp[order_eq_0]
+QED
+
+Theorem order_thm:
+  !m x n. 0 < n ⇒
+          (tord x = n ⇔ monoid_exp m x n = tmid m /\
+                        !p. 0 < p /\ p < n ⇒ monoid_exp m x p <> tmid m)
+Proof
+  xfer_back_tac [] >> simp[order_thm]
+QED
+
+Theorem monoid_order_id[simp]:
+  !m. tord (tmid m) = 1
+Proof
+  xfer_back_tac [] >> simp[monoid_order_id]
+QED
+
+Theorem monoid_order_eq_1:
+  !m x. x ∈ tmcarrier m ⇒ (tord x = 1 ⇔ x = tmid m)
+Proof
+  xfer_back_tac [] >> simp[monoid_order_eq_1]
+QED
+
+Theorem monoid_order_condition:
+  !m x. x ∈ tmcarrier m ⇒ !p. monoid_exp m x p = tmid m ⇔ tord x divides p
+Proof
+  xfer_back_tac [] >> simp[monoid_order_condition]
+QED
+
+Theorem monoid_order_power_eq_0:
+  !m x. x ∈ tmcarrier m ⇒ !k. tord (monoid_exp m x k) = 0 ⇔ 0 < k /\ tord x = 0
+Proof
+  xfer_back_tac[] >> simp[monoid_order_power_eq_0]
+QED
+
+Theorem monoid_order_power:
+  !m x. x ∈ tmcarrier m ⇒ !k. tord (monoid_exp m x k) * gcd (tord x) k = tord x
+Proof
+  xfer_back_tac[] >> simp[monoid_order_power]
+QED
+
+Theorem monoid_order_power_eqn:
+  !m x k. x ∈ tmcarrier m /\ 0 < k ⇒
+          tord (monoid_exp m x k) = tord x DIV gcd k (tord x)
+Proof
+  xfer_back_tac[] >> simp[monoid_order_power_eqn]
+QED
+
+Theorem monoid_order_power_coprime:
+  !m x k. x ∈ tmcarrier m /\ coprime k (tord x) ⇒
+          tord (monoid_exp m x k) = tord x
+Proof
+  xfer_back_tac[] >> simp[monoid_order_power_coprime]
+QED
+
+Theorem monoid_order_cofactor:
+  !m x n. x ∈ tmcarrier m /\ 0 < tord x /\ n divides tord x ⇒
+          tord (monoid_exp m x (tord x DIV n)) = n
+Proof
+  xfer_back_tac[] >> simp[monoid_order_cofactor]
+QED
+
+Theorem monoid_order_divisor:
+  !m x n. x ∈ tmcarrier m /\ 0 < tord x /\ n divides tord x ⇒
+          ∃y. y ∈ tmcarrier m /\ tord y = n
+Proof
+  xfer_back_tac[] >> simp[] >> metis_tac[monoid_order_divisor]
+QED
+
+Theorem monoid_order_common:
+  !m x y. x ∈ tmcarrier m /\ y ∈ tmcarrier m /\ tmop m x y = tmop m y x ⇒
+          ∃z. z ∈ tmcarrier m /\
+              tord z * gcd (tord x) (tord y) = lcm (tord x) (tord y)
+Proof
+  xfer_back_tac[] >> simp[] >>
+  metis_tac[monoid_order_common, arithmeticTheory.MULT_COMM]
+QED
+
+Theorem monoid_order_common_coprime:
+  !m x y. x ∈ tmcarrier m /\ y ∈ tmcarrier m /\ tmop m x y = tmop m y x /\
+          coprime (tord x) (tord y) ⇒
+          ∃z. z ∈ tmcarrier m /\ tord z = tord x * tord y
+Proof
+  xfer_back_tac[] >> simp[] >> metis_tac[monoid_order_common_coprime]
+QED
+
+Theorem monoid_exp_mod_order:
+  !m x n. x ∈ tmcarrier m /\ 0 < tord x ⇒
+          monoid_exp m x n = monoid_exp m x (n MOD tord x)
+Proof
+  xfer_back_tac[] >> simp[] >> metis_tac[monoid_exp_mod_order]
+QED
 
 val _ = export_theory();
